theories/AddSubLt.v
@@ -11,7 +11,7 @@ Section fundamental.
   Notation R := ((leibnizO Reg) -n> iProp Σ).
   Implicit Types w : (leibnizO Word).
   Implicit Types interp : D.
-
+(*
   Lemma RX_Add_Sub_Lt_case:
     ∀ E0 r a g fs fr b e p' w dst r1 r2
       (* RWX case *)
@@ -810,5 +810,6 @@ Section fundamental.
       exact (inl 0%Z). exact (inl 0%Z). exact (inl 0%Z). exact (inl 0%Z).
   Qed.*)
     Admitted. 
+*)
 
 End fundamental.
